formal/inference/Code_Generation.thy
@@ -474,7 +474,7 @@ definition logStates :: "nat \<Rightarrow> nat \<Rightarrow> unit" where
 (* This is the infer function but with logging *)
 function infer_with_log :: "nat \<Rightarrow> nat \<Rightarrow> iEFSM \<Rightarrow> strategy \<Rightarrow> update_modifier \<Rightarrow> (transition_matrix \<Rightarrow> bool) \<Rightarrow> (iEFSM \<Rightarrow> nondeterministic_pair fset) \<Rightarrow> iEFSM" where
   "infer_with_log stepNo k e r m check np = (
-    case inference_step e (rev (sorted_list_of_fset (k_score k e r))) m check np of
+    case inference_step e (sorted_list_of_fset (k_score k e r)) m check np of
       None \<Rightarrow> e |
       Some new \<Rightarrow> let 
         temp = iEFSM2dot new stepNo;
